code/array-secure.java
@@ -1,0 +1,6 @@
+int[] arr = new int[5];
+arr[0] = secret;
+if (arr[0] == 42)
+  println("checked");
+else
+  println("checked");
