code/bool-insecure.java
@@ -1,0 +1,3 @@
+boolean ret;
+ret = (high && true);
+return ret;
