code/bool-secure.java
@@ -1,0 +1,4 @@
+boolean ret;
+ret = (high || true) ||
+      (high || false);
+return ret;
