code/example.ml
@@ -1,0 +1,28 @@
+open Message
+
+let rec to_int (n:nat) : int =
+  match n with
+  | O -> 0 
+  | S n' -> 1 + to_int n'
+;;
+
+let n7 = S (S (S (S (S (S (S O))))))
+let n6 = S (S (S (S (S (S O)))))
+let n5 = S (S (S (S (S O))))
+let n4 = S (S (S (S O)))
+let n3 = S (S (S O)) 
+let n2 = S (S O)
+let n1 = S O
+
+let pb = Pair (Pair (n5, n1), n4)
+let pc = Pair (Pair (n7, n3), n6)
+
+let ()=
+  Printf.printf "B sends %i ==> C got A=%i and B=(%i, %i, %i)\n" 
+  (to_int (send pb)) (to_int (recv pc (send pb))) 
+  ((to_int (fst (fst pb)))) ((to_int (snd (fst pb)))) ((to_int (snd pb)))
+
+let ()=
+  Printf.printf "C sends %i ==> B got A=%i and C=(%i, %i, %i)\n" 
+  (to_int (send pc)) (to_int (recv pb (send pc))) 
+  ((to_int (fst (fst pc)))) ((to_int (snd (fst pc)))) ((to_int (snd pc)))
