code/loop-insecure.java
@@ -1,0 +1,4 @@
+int f(int h, int l) {
+  while (h>0) { h--; l++; }
+  return l;
+}
