code/message.ml
@@ -1,0 +1,327 @@
+
+type __ = Obj.t
+let __ = let rec f _ = Obj.repr f in Obj.repr f
+
+type bool =
+| True
+| False
+
+(** val negb : bool -> bool **)
+
+let negb = function
+| True -> False
+| False -> True
+
+type nat =
+| O
+| S of nat
+
+type ('a, 'b) prod =
+| Pair of 'a * 'b
+
+(** val fst : ('a1, 'a2) prod -> 'a1 **)
+
+let fst = function
+| Pair (x, _) -> x
+
+(** val snd : ('a1, 'a2) prod -> 'a2 **)
+
+let snd = function
+| Pair (_, y) -> y
+
+type 'a list =
+| Nil
+| Cons of 'a * 'a list
+
+(** val pred : nat -> nat **)
+
+let pred n = match n with
+| O -> n
+| S u0 -> u0
+
+(** val add : nat -> nat -> nat **)
+
+let rec add n m =
+  match n with
+  | O -> m
+  | S p -> S (add p m)
+
+(** val sub : nat -> nat -> nat **)
+
+let rec sub n m =
+  match n with
+  | O -> n
+  | S k -> (match m with
+            | O -> n
+            | S l0 -> sub k l0)
+
+type reflect =
+| ReflectT
+| ReflectF
+
+(** val iffP : bool -> reflect -> reflect **)
+
+let iffP _ pb =
+  let _evar_0_ = fun _ _ _ -> ReflectT in
+  let _evar_0_0 = fun _ _ _ -> ReflectF in
+  (match pb with
+   | ReflectT -> _evar_0_ __ __ __
+   | ReflectF -> _evar_0_0 __ __ __)
+
+(** val idP : bool -> reflect **)
+
+let idP = function
+| True -> ReflectT
+| False -> ReflectF
+
+type 't pred0 = 't -> bool
+
+type 't predType =
+  __ -> 't pred0
+  (* singleton inductive, whose constructor was PredType *)
+
+type 't pred_sort = __
+
+type 't rel = 't -> 't pred0
+
+type 't mem_pred =
+  't pred0
+  (* singleton inductive, whose constructor was Mem *)
+
+(** val pred_of_mem : 'a1 mem_pred -> 'a1 pred_sort **)
+
+let pred_of_mem mp =
+  Obj.magic mp
+
+(** val in_mem : 'a1 -> 'a1 mem_pred -> bool **)
+
+let in_mem x mp =
+  Obj.magic pred_of_mem mp x
+
+(** val mem : 'a1 predType -> 'a1 pred_sort -> 'a1 mem_pred **)
+
+let mem pT =
+  pT
+
+type 't eq_axiom = 't -> 't -> reflect
+
+module Coq_hasDecEq =
+ struct
+  type 't axioms_ = { eq_op : 't rel; eqP : 't eq_axiom }
+
+  (** val eq_op : 'a1 axioms_ -> 'a1 rel **)
+
+  let eq_op record =
+    record.eq_op
+ end
+
+module Equality =
+ struct
+  type 't axioms_ =
+    't Coq_hasDecEq.axioms_
+    (* singleton inductive, whose constructor was Class *)
+
+  (** val eqtype_hasDecEq_mixin : 'a1 axioms_ -> 'a1 Coq_hasDecEq.axioms_ **)
+
+  let eqtype_hasDecEq_mixin record =
+    record
+
+  type coq_type =
+    __ axioms_
+    (* singleton inductive, whose constructor was Pack *)
+
+  type sort = __
+
+  (** val coq_class : coq_type -> sort axioms_ **)
+
+  let coq_class record =
+    record
+ end
+
+(** val eq_op0 : Equality.coq_type -> Equality.sort rel **)
+
+let eq_op0 s =
+  (Equality.eqtype_hasDecEq_mixin (Equality.coq_class s)).Coq_hasDecEq.eq_op
+
+(** val eqn : nat -> nat -> bool **)
+
+let rec eqn m n =
+  match m with
+  | O -> (match n with
+          | O -> True
+          | S _ -> False)
+  | S m' -> (match n with
+             | O -> False
+             | S n' -> eqn m' n')
+
+(** val eqnP : nat eq_axiom **)
+
+let eqnP n m =
+  iffP (eqn n m) (idP (eqn n m))
+
+(** val hB_unnamed_factory_1 : nat Coq_hasDecEq.axioms_ **)
+
+let hB_unnamed_factory_1 =
+  { Coq_hasDecEq.eq_op = eqn; Coq_hasDecEq.eqP = eqnP }
+
+(** val datatypes_nat__canonical__eqtype_Equality : Equality.coq_type **)
+
+let datatypes_nat__canonical__eqtype_Equality =
+  Obj.magic hB_unnamed_factory_1
+
+(** val addn_rec : nat -> nat -> nat **)
+
+let addn_rec =
+  add
+
+(** val addn : nat -> nat -> nat **)
+
+let addn =
+  addn_rec
+
+(** val subn_rec : nat -> nat -> nat **)
+
+let subn_rec =
+  sub
+
+(** val subn : nat -> nat -> nat **)
+
+let subn =
+  subn_rec
+
+(** val leq : nat -> nat -> bool **)
+
+let leq m n =
+  eq_op0 datatypes_nat__canonical__eqtype_Equality (Obj.magic subn m n)
+    (Obj.magic O)
+
+(** val nth : 'a1 -> 'a1 list -> nat -> 'a1 **)
+
+let rec nth x0 s n =
+  match s with
+  | Nil -> x0
+  | Cons (x, s') -> (match n with
+                     | O -> x
+                     | S n' -> nth x0 s' n')
+
+(** val filter : 'a1 pred0 -> 'a1 list -> 'a1 list **)
+
+let rec filter a = function
+| Nil -> Nil
+| Cons (x, s') ->
+  (match a x with
+   | True -> Cons (x, (filter a s'))
+   | False -> filter a s')
+
+(** val mem_seq :
+    Equality.coq_type -> Equality.sort list -> Equality.sort -> bool **)
+
+let rec mem_seq t = function
+| Nil -> (fun _ -> False)
+| Cons (y, s') ->
+  let p = mem_seq t s' in
+  (fun x -> match eq_op0 t x y with
+            | True -> True
+            | False -> p x)
+
+type seq_eqclass = Equality.sort list
+
+(** val pred_of_seq :
+    Equality.coq_type -> seq_eqclass -> Equality.sort pred_sort **)
+
+let pred_of_seq t s =
+  Obj.magic mem_seq t s
+
+(** val seq_predType : Equality.coq_type -> Equality.sort predType **)
+
+let seq_predType t =
+  Obj.magic pred_of_seq t
+
+(** val iota : nat -> nat -> nat list **)
+
+let rec iota m = function
+| O -> Nil
+| S n' -> Cons (m, (iota (S m) n'))
+
+(** val foldr : ('a1 -> 'a2 -> 'a2) -> 'a2 -> 'a1 list -> 'a2 **)
+
+let rec foldr f z0 = function
+| Nil -> z0
+| Cons (x, s') -> f x (foldr f z0 s')
+
+(** val sumn : nat list -> nat **)
+
+let sumn =
+  foldr addn O
+
+(** val modn_rec : nat -> nat -> nat **)
+
+let rec modn_rec d m =
+  match subn m d with
+  | O -> m
+  | S m' -> modn_rec d m'
+
+(** val modn : nat -> nat -> nat **)
+
+let modn m d =
+  match leq (S O) d with
+  | True -> modn_rec (pred d) m
+  | False -> m
+
+(** val u : nat list **)
+
+let u =
+  iota (S O) (S (S (S (S (S (S (S O)))))))
+
+(** val l : ((nat, nat) prod, nat) prod -> nat list **)
+
+let l t =
+  Cons ((fst (fst t)), (Cons ((snd (fst t)), (Cons ((snd t), Nil)))))
+
+(** val t3 : nat list -> ((nat, nat) prod, nat) prod **)
+
+let t3 l0 =
+  Pair ((Pair ((nth O l0 O), (nth O l0 (S O)))), (nth O l0 (S (S O))))
+
+(** val outside : nat list -> Equality.sort list **)
+
+let outside s =
+  filter (fun x ->
+    negb
+      (in_mem x
+        (mem (seq_predType datatypes_nat__canonical__eqtype_Equality)
+          (Obj.magic s)))) (Obj.magic u)
+
+(** val encode : nat -> nat -> nat -> nat -> nat **)
+
+let encode n1 n2 n3 x =
+  let r =
+    modn
+      (addn
+        (sumn (Obj.magic outside (Cons (n1, (Cons (n2, (Cons (n3, Nil))))))))
+        x) (S (S (S (S (S (S (S O)))))))
+  in
+  (match eq_op0 datatypes_nat__canonical__eqtype_Equality (Obj.magic r)
+           (Obj.magic O) with
+   | True -> S (S (S (S (S (S (S O))))))
+   | False -> r)
+
+(** val send : ((nat, nat) prod, nat) prod -> nat **)
+
+let send t =
+  encode (fst (fst t)) (snd (fst t)) (snd t) (S (S (S (S (S (S (S O)))))))
+
+(** val recv : ((nat, nat) prod, nat) prod -> nat -> nat **)
+
+let recv t m =
+  encode (fst (fst t)) (snd (fst t)) (snd t) m
+
+(** val recover :
+    ((nat, nat) prod, nat) prod -> nat -> ((nat, nat) prod, nat) prod **)
+
+let recover t n =
+  t3
+    (filter (fun x ->
+      negb
+        (eq_op0 datatypes_nat__canonical__eqtype_Equality (Obj.magic x)
+          (Obj.magic recv t n))) (Obj.magic outside (l t)))
