code/leftpad.dfy
@@ -1,30 +1,31 @@
-function method max(a: int, b: int): int
+function Max(a: int, b: int): int
 {
-    if a > b then a else b
+  if a > b then a else b
 }
 
-method LeftPad(c: char, n: int, s: seq<char>) returns (v: seq<char>)
-ensures |v| == max(n, |s|)
-ensures forall i :: 0 <= i < n - |s| ==> v[i] == c
-ensures forall i :: 0 <= i < |s| ==> v[max(n - |s|, 0)+i] == s[i]
+method LeftPad(c: char, n: int, s: seq<char>)
+  returns (v: seq<char>)
+  ensures |v| == Max(n, |s|)
+  ensures forall i :: 0 <= i < n - |s| ==> v[i] == c
+  ensures forall i :: 0 <= i < |s| ==> v[Max(n - |s|, 0) + i] == s[i]
 {
-
-    var pad, i := max(n - |s|, 0), 0;
-    v := s;
-    while i < pad decreases pad - i
+  var pad, i := Max(n - |s|, 0), 0;
+  v := s;
+  while i < pad
     invariant 0 <= i <= pad
     invariant |v| == |s| + i
     invariant forall j :: 0 <= j < i ==> v[j] == c
-    invariant forall j :: 0 <= j < |s| ==> v[i+j] == s[j]
-    {
-        v := [c] + v;
-        i := i + 1;
-    }
+    invariant forall j :: 0 <= j < |s| ==> v[i + j] == s[j]
+    decreases pad - i
+  {
+    v := [c] + v;
+    i := i + 1;
+  }
 }
 
 method Main() {
-    var l1 := LeftPad('0', 5, "foo");
-    var l2 := LeftPad('0', 1, "foo");
-    print l1 + "\n\n";
-    print l2;
+  var l1 := LeftPad('0', 5, "foo");
+  var l2 := LeftPad('0', 1, "foo");
+  print l1 + "\n\n";
+  print l2;
 }
