code/equiv.dfy
@@ -1,0 +1,11 @@
+type bit = i: nat | i <= 1 witness 1
+
+function Program2 (b : bit, X : nat, Y : nat) : nat {
+  X * b + Y * (1 - b)
+}
+
+method Program1 (b : bit, X : nat, Y : nat) returns (Z: nat)
+  ensures Z == Program2(b, X, Y) {
+  if b == 1 { Z := X; }
+  else { Z := Y; }
+}
