code/equiv.v
@@ -1,0 +1,33 @@
+Require Import Maps Imp.
+From Coq Require Import Arith.PeanoNat. Import Nat.
+From Coq Require Import Arith.EqNat.
+
+Open Scope com_scope.
+
+Definition aequiv (a1 a2 : aexp) : Prop :=
+  forall (st : state),  aeval st a1 = aeval st a2.
+
+Definition equiv (c1 c2 : com) : Prop :=
+  forall (st st' : state), (st =[ c1 ]=> st') <-> (st =[ c2 ]=> st').
+
+Notation "p '===' q" :=
+  (cequiv p q) (at level 50, left associativity).
+
+Theorem prog_eq b X Y Z :
+    b = 0 \/ b = 1 ->
+    <{ if b = 1 then Z := X else Z := Y end }>
+    === <{ Z := X * b + Y * (1 - b) }>.
+Proof.
+  intros; split.
+  (* if ... *)
+  - intros C1; inversion C1; subst; clear C1;
+      inversion H; subst; try discriminate;
+      inversion H6; subst; apply E_Asgn; simpl;
+      rewrite mul_0_r, mul_1_r; auto.
+  (* Z := ... *)
+  - intros C2; destruct H as [H|H]; subst;
+      [apply E_IfFalse|apply E_IfTrue]; auto;
+      inversion C2; subst; clear C2;
+      apply E_Asgn; simpl;
+      rewrite mul_0_r, mul_1_r; auto.
+Qed.    
