code/leftpad-ssrefl.v
@@ -8,7 +8,7 @@ Section LeftPad.
 
 (* [def] is the default value, i.e. type T is not empty *)
 Variables (T : Type) (def : T).
-Local Notation nth := (nth def)  (* access n-th element of the input list *)
+Local Notation nth := (nth def)  (* n-th element of list *)
 
 Definition leftpad (c : T) (n : nat) (s : seq T) : seq T :=
   ncons (n - size s) c s.
@@ -21,8 +21,8 @@ Lemma prefix_spec c n s :
   forall i, i < n - size s -> nth (leftpad c n s) i = c.
 Proof. by move=> i; rewrite nth_ncons => ->. Qed.
 
-Lemma suffix_spec c n s :
-  forall i, i < size s -> nth (leftpad c n s) (n - size s + i) = nth s i.
+Lemma suffix_spec c n s : forall i,
+  i < size s -> nth (leftpad c n s) (n - size s + i) = nth s i.
 Proof. by move=> i _; rewrite nth_ncons addKn ifN // -ltnNge leq_addr. Qed.
 
 End LeftPad.
